verified_quicksort_array.ml
@@ -1,0 +1,291 @@
+
+type ('a, 'b) prod =
+| Pair of 'a * 'b
+
+(** val snd : ('a1, 'a2) prod -> 'a2 **)
+
+let snd = function
+| Pair (_, y) -> y
+
+(** val length : 'a1 Array.array -> int **)
+
+let rec length = function
+| [||] -> 0
+| _::l' -> (fun x -> x + 1) (length l')
+
+type ('a, 'p) sigT =
+| ExistT of 'a * 'p
+
+(** val projT1 : ('a1, 'a2) sigT -> 'a1 **)
+
+let projT1 = function
+| ExistT (a, _) -> a
+
+(** val projT2 : ('a1, 'a2) sigT -> 'a2 **)
+
+let projT2 = function
+| ExistT (_, h) -> h
+
+(** val add : int -> int -> int **)
+
+let rec add = ( + )
+
+(** val mul : int -> int -> int **)
+
+let rec mul = ( - )
+
+(** val sub : int -> int -> int **)
+
+let rec sub = ( - )
+
+module Nat =
+ struct
+  (** val sub : int -> int -> int **)
+
+  let rec sub n m =
+    (fun zero succ n ->
+
+ if n=0 then zero ()
+
+ else succ (n-1))
+      (fun _ -> n)
+      (fun k ->
+      (fun zero succ n ->
+
+ if n=0 then zero ()
+
+ else succ (n-1))
+        (fun _ -> n)
+        (fun l -> sub k l)
+        m)
+      n
+
+  (** val divmod : int -> int -> int -> int -> (int, int) prod **)
+
+  let rec divmod x y q u =
+    (fun zero succ n ->
+
+ if n=0 then zero ()
+
+ else succ (n-1))
+      (fun _ -> Pair (q, u))
+      (fun x' ->
+      (fun zero succ n ->
+
+ if n=0 then zero ()
+
+ else succ (n-1))
+        (fun _ -> divmod x' y ((fun x -> x + 1) q) y)
+        (fun u' -> divmod x' y q u')
+        u)
+      x
+
+  (** val modulo : int -> int -> int **)
+
+  let modulo x y =
+    (fun zero succ n ->
+
+ if n=0 then zero ()
+
+ else succ (n-1))
+      (fun _ -> x)
+      (fun y' -> sub y' (snd (divmod x y' 0 y')))
+      y
+ end
+
+(** val fold_left : ('a1 -> 'a2 -> 'a1) -> 'a2 Array.array -> 'a1 -> 'a1 **)
+
+let rec fold_left f l a0 =
+  match l with
+  | [||] -> a0
+  | b::t -> fold_left f t (f a0 b)
+
+(** val lookup : int Array.array -> int -> int **)
+
+let rec lookup l i =
+  match l with
+  | [||] -> 0
+  | h::t -> if (<=) i 0 then h else lookup t (sub i ((fun x -> x + 1) 0))
+
+(** val insert : int -> int -> int Array.array -> int Array.array **)
+
+let rec insert elem index l =
+  (fun zero succ n ->
+
+ if n=0 then zero ()
+
+ else succ (n-1))
+    (fun _ -> match l with
+              | [||] -> elem::[||]
+              | _::xs -> elem::xs)
+    (fun _ ->
+    match l with
+    | [||] -> elem::[||]
+    | x::xs -> x::(insert elem (sub index ((fun x -> x + 1) 0)) xs))
+    index
+
+(** val randnat : int -> int -> int **)
+
+let randnat seed bound =
+  Nat.modulo
+    (add
+      (mul seed ((fun x -> x + 1) ((fun x -> x + 1) ((fun x -> x + 1)
+        ((fun x -> x + 1) ((fun x -> x + 1) ((fun x -> x + 1)
+        ((fun x -> x + 1) ((fun x -> x + 1) ((fun x -> x + 1)
+        ((fun x -> x + 1) ((fun x -> x + 1) ((fun x -> x + 1)
+        ((fun x -> x + 1) ((fun x -> x + 1) ((fun x -> x + 1)
+        ((fun x -> x + 1) ((fun x -> x + 1) ((fun x -> x + 1)
+        ((fun x -> x + 1) ((fun x -> x + 1) ((fun x -> x + 1)
+        ((fun x -> x + 1) ((fun x -> x + 1) ((fun x -> x + 1)
+        ((fun x -> x + 1) ((fun x -> x + 1) ((fun x -> x + 1)
+        ((fun x -> x + 1) ((fun x -> x + 1) ((fun x -> x + 1)
+        ((fun x -> x + 1) 0)))))))))))))))))))))))))))))))) ((fun x -> x + 1)
+      ((fun x -> x + 1) ((fun x -> x + 1) ((fun x -> x + 1) ((fun x -> x + 1)
+      ((fun x -> x + 1) ((fun x -> x + 1) 0)))))))) bound
+
+(** val fst3 : ((int Array.array, int) prod, int) prod -> int Array.array **)
+
+let fst3 = function
+| Pair (p, _) -> let Pair (a, _) = p in a
+
+(** val swap : int Array.array -> int -> int -> int Array.array **)
+
+let swap l i1 i2 =
+  insert (lookup l i2) i1 (insert (lookup l i1) i2 l)
+
+(** val shuffle : int Array.array -> int Array.array **)
+
+let shuffle l =
+  fst3
+    (fold_left (fun acc _ ->
+      let Pair (p, point) = acc in
+      let Pair (li, seed) = p in
+      Pair ((Pair ((swap li point (randnat seed (length li))),
+      (add seed ((fun x -> x + 1) 0)))), (add point ((fun x -> x + 1) 0)))) l
+      (Pair ((Pair (l, ((fun x -> x + 1) ((fun x -> x + 1) ((fun x -> x + 1)
+      ((fun x -> x + 1) ((fun x -> x + 1) ((fun x -> x + 1) ((fun x -> x + 1)
+      ((fun x -> x + 1) ((fun x -> x + 1) ((fun x -> x + 1) ((fun x -> x + 1)
+      ((fun x -> x + 1) ((fun x -> x + 1) ((fun x -> x + 1) ((fun x -> x + 1)
+      ((fun x -> x + 1) ((fun x -> x + 1) ((fun x -> x + 1) ((fun x -> x + 1)
+      ((fun x -> x + 1) ((fun x -> x + 1) ((fun x -> x + 1) ((fun x -> x + 1)
+      ((fun x -> x + 1) ((fun x -> x + 1) ((fun x -> x + 1) ((fun x -> x + 1)
+      ((fun x -> x + 1) ((fun x -> x + 1) ((fun x -> x + 1) ((fun x -> x + 1)
+      ((fun x -> x + 1) ((fun x -> x + 1) ((fun x -> x + 1) ((fun x -> x + 1)
+      ((fun x -> x + 1) ((fun x -> x + 1) ((fun x -> x + 1) ((fun x -> x + 1)
+      ((fun x -> x + 1) ((fun x -> x + 1) ((fun x -> x + 1)
+      0)))))))))))))))))))))))))))))))))))))))))))), 0)))
+
+(** val partition_left_func :
+    (int Array.array, (int, (int, int) sigT) sigT) sigT -> int **)
+
+let rec partition_left_func x =
+  let l = projT1 x in
+  let pivot = projT1 (projT2 x) in
+  let lo = projT1 (projT2 (projT2 x)) in
+  let hi = projT2 (projT2 (projT2 x)) in
+  let partition_left0 = fun l0 pivot0 lo0 hi0 ->
+    partition_left_func (ExistT (l0, (ExistT (pivot0, (ExistT (lo0, hi0))))))
+  in
+  let filtered_var = (<=) hi lo in
+  if filtered_var
+  then lo
+  else let filtered_var0 = (<=) (lookup l lo) pivot in
+       if filtered_var0
+       then partition_left0 l pivot (add lo ((fun x -> x + 1) 0)) hi
+       else lo
+
+(** val partition_left : int Array.array -> int -> int -> int -> int **)
+
+let partition_left l pivot lo hi =
+  partition_left_func (ExistT (l, (ExistT (pivot, (ExistT (lo, hi))))))
+
+(** val partition_right_func :
+    (int Array.array, (int, (int, int) sigT) sigT) sigT -> int **)
+
+let rec partition_right_func x =
+  let l = projT1 x in
+  let pivot = projT1 (projT2 x) in
+  let lo = projT1 (projT2 (projT2 x)) in
+  let hi = projT2 (projT2 (projT2 x)) in
+  let partition_right0 = fun l0 pivot0 lo0 hi0 ->
+    partition_right_func (ExistT (l0, (ExistT (pivot0, (ExistT (lo0, hi0))))))
+  in
+  let filtered_var = (<=) hi lo in
+  if filtered_var
+  then hi
+  else let filtered_var0 = (<=) pivot (lookup l hi) in
+       if filtered_var0
+       then partition_right0 l pivot lo (sub hi ((fun x -> x + 1) 0))
+       else hi
+
+(** val partition_right : int Array.array -> int -> int -> int -> int **)
+
+let partition_right l pivot lo hi =
+  partition_right_func (ExistT (l, (ExistT (pivot, (ExistT (lo, hi))))))
+
+(** val partition_func :
+    (int Array.array, (int, (int, (int, int) sigT) sigT) sigT) sigT -> (int,
+    int Array.array) prod **)
+
+let rec partition_func x =
+  let l = projT1 x in
+  let pivot = projT1 (projT2 x) in
+  let lo = projT1 (projT2 (projT2 x)) in
+  let initial_lo = projT1 (projT2 (projT2 (projT2 x))) in
+  let hi = projT2 (projT2 (projT2 (projT2 x))) in
+  let partition0 = fun l0 pivot0 lo0 initial_lo0 hi0 ->
+    partition_func (ExistT (l0, (ExistT (pivot0, (ExistT (lo0, (ExistT
+      (initial_lo0, hi0))))))))
+  in
+  let filtered_var = Pair ((partition_left l pivot lo hi),
+    (partition_right l pivot lo hi))
+  in
+  let Pair (i, j) = filtered_var in
+  let filtered_var0 = (<=) j i in
+  if filtered_var0
+  then Pair (j, (swap l initial_lo j))
+  else let filtered_var1 = (<=) j hi in
+       if filtered_var1
+       then let filtered_var2 = (<=) lo i in
+            if filtered_var2
+            then partition0 (swap l i j) pivot i initial_lo j
+            else Pair (j, l)
+       else Pair (j, l)
+
+(** val partition :
+    int Array.array -> int -> int -> int -> int -> (int, int Array.array) prod **)
+
+let partition l pivot lo initial_lo hi =
+  partition_func (ExistT (l, (ExistT (pivot, (ExistT (lo, (ExistT
+    (initial_lo, hi))))))))
+
+(** val sort_func :
+    (int Array.array, (int, int) sigT) sigT -> int Array.array **)
+
+let rec sort_func x =
+  let l = projT1 x in
+  let lo = projT1 (projT2 x) in
+  let hi = projT2 (projT2 x) in
+  let sort0 = fun l0 lo0 hi0 -> sort_func (ExistT (l0, (ExistT (lo0, hi0))))
+  in
+  let filtered_var = (<=) hi lo in
+  if filtered_var
+  then l
+  else let filtered_var0 = partition l (lookup l lo) lo lo hi in
+       let Pair (j, partitioned) = filtered_var0 in
+       let filtered_var1 = if (<=) j hi then (<=) lo j else false in
+       if filtered_var1
+       then sort0 (sort0 partitioned lo (sub j ((fun x -> x + 1) 0)))
+              (add j ((fun x -> x + 1) 0)) hi
+       else [||]
+
+(** val sort : int Array.array -> int -> int -> int Array.array **)
+
+let sort l lo hi =
+  sort_func (ExistT (l, (ExistT (lo, hi))))
+
+(** val quicksort : int Array.array -> int Array.array **)
+
+let quicksort l =
+  let shuffled = shuffle l in
+  sort shuffled 0 (sub (length shuffled) ((fun x -> x + 1) 0))
