verified_quicksort_array.mli
@@ -1,0 +1,66 @@
+
+type ('a, 'b) prod =
+| Pair of 'a * 'b
+
+val snd : ('a1, 'a2) prod -> 'a2
+
+val length : 'a1 Array.array -> int
+
+type ('a, 'p) sigT =
+| ExistT of 'a * 'p
+
+val projT1 : ('a1, 'a2) sigT -> 'a1
+
+val projT2 : ('a1, 'a2) sigT -> 'a2
+
+val add : int -> int -> int
+
+val mul : int -> int -> int
+
+val sub : int -> int -> int
+
+module Nat :
+ sig
+  val sub : int -> int -> int
+
+  val divmod : int -> int -> int -> int -> (int, int) prod
+
+  val modulo : int -> int -> int
+ end
+
+val fold_left : ('a1 -> 'a2 -> 'a1) -> 'a2 Array.array -> 'a1 -> 'a1
+
+val lookup : int Array.array -> int -> int
+
+val insert : int -> int -> int Array.array -> int Array.array
+
+val randnat : int -> int -> int
+
+val fst3 : ((int Array.array, int) prod, int) prod -> int Array.array
+
+val swap : int Array.array -> int -> int -> int Array.array
+
+val shuffle : int Array.array -> int Array.array
+
+val partition_left_func :
+  (int Array.array, (int, (int, int) sigT) sigT) sigT -> int
+
+val partition_left : int Array.array -> int -> int -> int -> int
+
+val partition_right_func :
+  (int Array.array, (int, (int, int) sigT) sigT) sigT -> int
+
+val partition_right : int Array.array -> int -> int -> int -> int
+
+val partition_func :
+  (int Array.array, (int, (int, (int, int) sigT) sigT) sigT) sigT -> (int,
+  int Array.array) prod
+
+val partition :
+  int Array.array -> int -> int -> int -> int -> (int, int Array.array) prod
+
+val sort_func : (int Array.array, (int, int) sigT) sigT -> int Array.array
+
+val sort : int Array.array -> int -> int -> int Array.array
+
+val quicksort : int Array.array -> int Array.array
